Instance of Lts, LtsEq, LtsOba

theories/ACCS_with_ValuePassing_Instance.v
@@ -55,12 +55,23 @@ Notation "c ⋉ v" := (act c v) (at level 50).
 
 
 Inductive Equation (A : Type) : Type :=
-| Equality : A -> A -> Equation A.
+| tt : Equation A
+| ff : Equation A
+| Inequality : A -> A -> Equation A
+| Or : Equation A -> Equation A -> Equation A
+| Not : Equation A -> Equation A.
 
-Arguments  Equality {_} _ _.
+Arguments  tt  {_}.
+Arguments  ff  {_} .
+Arguments  Inequality  {_} _ _.
+Arguments  Or  {_} _ _.
+Arguments  Not  {_}  _.
 
-Notation "x == y" := (Equality x y) (at level 50).
+Notation "'non' e" := (Not e) (at level 50).
+Notation "x ∨ y" := (Or x y).
+Notation "x ⩽ y" := (Inequality x y) (at level 50).
 
+Parameter Eval_Eq : Equation Data -> (option bool).
 
 (* Definition of processes*)
 Inductive proc : Type :=
@@ -116,11 +127,14 @@ match Y with
 | bvar i => if (decide(i = k)) then X else bvar i
 end.
 
-Definition subst_in_Equation (k : nat) (X : Data) (E : Equation Data) : Equation Data :=
-match E with 
-| D1 == D2 => (subst_Data k X D1) == (subst_Data k X D2)
+Fixpoint subst_in_Equation (k : nat) (X : Data) (E : Equation Data) : Equation Data :=
+match E with
+| tt => tt
+| ff => ff
+| D1 ⩽ D2 => (subst_Data k X D1) ⩽ (subst_Data k X D2)
+| e1 ∨ e2 => (subst_in_Equation k X e1) ∨ (subst_in_Equation k X e2)
+| non e => non (subst_in_Equation k X e)
 end.
-
 
 Fixpoint subst_in_proc (k : nat) (X : Data) (p : proc) {struct p} : proc :=
 match p with
@@ -168,28 +182,28 @@ end.
 Inductive lts : proc-> (Act TypeOfActions) -> proc -> Prop :=
 (*The Input and the Output*)
 | lts_input : forall {c v P},
-    lts (c ? x • P) (ActIn (c ⋉ (cst v))) (P^v)
+    lts (c ? x • P) (ActIn (c ⋉ v)) (P^v)
 | lts_output : forall {c v},
-    lts (c ! (cst v) • 𝟘) (ActOut (c ⋉ (cst v))) 𝟘
+    lts (c ! v • 𝟘) (ActOut (c ⋉ v)) 𝟘
 
 (*The actions Tau*)
 | lts_tau : forall {P},
     lts (t • P) τ P
 | lts_recursion : forall {x P},
     lts (rec x • P) τ (pr_subst x P (rec x • P))
-| lts_ifOne : forall p q x y, x = y -> 
-    lts (If (x == y) Then p Else q) τ p
-| lts_ifZero : forall {p q x y}, ~(x = y) -> 
-    lts (If (x == y) Then p Else q) τ q
+| lts_ifOne : forall {p q E}, Eval_Eq E = Some true -> 
+    lts (If E Then p Else q) τ p
+| lts_ifZero : forall {p q E}, Eval_Eq E = Some false -> 
+    lts (If E Then p Else q) τ q
 
 (* Communication of a channel output and input that have the same name*)
 | lts_comL : forall {c v p1 p2 q1 q2},
-    lts p1 (ActOut (c ⋉ (cst v))) p2 ->
-    lts q1 (ActIn (c ⋉ (cst v))) q2 ->
+    lts p1 (ActOut (c ⋉ v)) p2 ->
+    lts q1 (ActIn (c ⋉ v)) q2 ->
     lts (p1 ‖ q1) τ (p2 ‖ q2) 
 | lts_comR : forall {c v p1 p2 q1 q2},
-    lts p1 (ActOut (c ⋉ (cst v))) p2 ->
-    lts q1 (ActIn (c ⋉ (cst v))) q2 ->
+    lts p1 (ActOut (c ⋉ v)) p2 ->
+    lts q1 (ActIn (c ⋉ v)) q2 ->
     lts (q1 ‖ p1) τ (q2 ‖ p2)
 
 (*The decoration for the transition system...*)
@@ -451,32 +465,14 @@ Qed.
 
 #[global] Hint Resolve cgr_par_nil cgr_par_nil_rev cgr_par_nil_rev cgr_par_com cgr_par_assoc 
 cgr_par_assoc_rev cgr_choice_nil cgr_choice_nil_rev cgr_choice_com cgr_choice_assoc 
-cgr_choice_assoc_rev cgr_recursion cgr_tau cgr_input cgr_par cgr_choice 
+cgr_choice_assoc_rev cgr_recursion cgr_tau cgr_input cgr_if_left cgr_if_right cgr_par cgr_choice 
 cgr_refl cgr_symm cgr_trans:cgr.
 
 
 Lemma Congruence_Respects_Substitution : forall p q v k, p ≡* q -> (subst_in_proc k v p) ≡* (subst_in_proc k v q).
 Proof.
 intros. revert k. revert v. dependent induction H. 
-* dependent induction H.
-  - reflexivity.
-  - eauto with cgr.
-  - eauto with cgr.
-  - simpl. eauto with cgr.
-  - simpl. eauto with cgr.
-  - simpl. eauto with cgr.
-  - simpl. eauto with cgr.
-  - simpl. eauto with cgr.
-  - simpl. eauto with cgr.
-  - simpl. eauto with cgr.
-  - simpl. eauto with cgr.
-  - simpl. eauto with cgr.
-  - simpl. eauto with cgr.
-  - simpl. intros. apply cgr_input. apply IHcgr_step. 
-  - simpl. eauto with cgr.
-  - simpl. intros. apply cgr_if_left.  auto. 
-  - simpl. intros. apply cgr_if_right. auto.
-  - simpl. eauto with cgr.
+* dependent induction H; simpl; eauto with cgr.
 * eauto with cgr.
 Qed.
 
@@ -489,13 +485,13 @@ induction p as (p & Hp) using
     (well_founded_induction (wf_inverse_image _ nat _ size Nat.lt_wf_0)).
 destruct p.
   - simpl. intro. apply cgr_fullpar.
-    apply Hp. simpl. rewrite <-Nat.add_succ_r. apply PeanoNat.Nat.lt_add_pos_r. apply Nat.lt_0_succ. exact H. 
-    apply Hp. simpl. rewrite <-Nat.add_succ_l. apply PeanoNat.Nat.lt_add_pos_l. apply Nat.lt_0_succ. exact H.
-  - simpl. intro. destruct (decide (x = n)). exact H. reflexivity.
-  - simpl. intro. destruct (decide (x = n)). reflexivity. apply cgr_recursion. apply Hp. simpl. auto. exact H.
+    apply Hp. simpl. auto with arith. assumption. 
+    apply Hp. simpl. auto with arith. assumption. 
+  - simpl. intro. destruct (decide (x = n)). assumption. reflexivity.
+  - simpl. intro. destruct (decide (x = n)). reflexivity. apply cgr_recursion. apply Hp. simpl. auto. assumption.
   - simpl. intro. apply cgr_full_if.
-    apply Hp. simpl. rewrite <-Nat.add_succ_r. apply PeanoNat.Nat.lt_add_pos_r. apply Nat.lt_0_succ. exact H. 
-    apply Hp. simpl. rewrite <-Nat.add_succ_l. apply PeanoNat.Nat.lt_add_pos_l. apply Nat.lt_0_succ. exact H.  
+    apply Hp. simpl. auto with arith. assumption. 
+    apply Hp. simpl. auto with arith. assumption.  
   - simpl. intros. eauto with cgr.
   - destruct g0.
     * intros. simpl. reflexivity.
@@ -503,8 +499,8 @@ destruct p.
     * intros. simpl. apply cgr_input. apply Hp. simpl. auto. auto.
     * intros. simpl. apply cgr_tau. apply Hp. simpl. auto. auto.
     * intros. simpl. apply cgr_fullchoice. 
-      assert (pr_subst x (g g0_1) q ≡* pr_subst x (g g0_1) q'). apply Hp. simpl. auto with arith. auto.
-      auto. assert (pr_subst x (g g0_2) q ≡* pr_subst x (g g0_2) q'). apply Hp. simpl. auto with arith. auto.
+      assert (pr_subst x (g g0_1) q ≡* pr_subst x (g g0_1) q'). apply Hp. simpl. auto with arith. assumption.
+      auto. assert (pr_subst x (g g0_2) q ≡* pr_subst x (g g0_2) q'). apply Hp. simpl. auto with arith. assumption.
       auto. 
 Qed.
 (* ≡ respects the substitution of his variable*)
@@ -512,18 +508,7 @@ Lemma cgr_step_subst2 : forall p p' q x, p ≡ p' → pr_subst x p q ≡ pr_subs
 Proof.
   induction p as (p & Hp) using
     (well_founded_induction (wf_inverse_image _ nat _ size Nat.lt_wf_0)).
-  intros p' q n hcgr ; inversion hcgr; try auto; try (exact H).
-  - constructor.
-  - constructor.
-  - constructor.
-  - constructor.
-  - constructor.
-  - constructor.
-  - constructor.
-  - constructor.
-  - constructor.
-  - constructor.
-  - constructor.
+  intros p' q n hcgr ; inversion hcgr; try auto; try (exact H); try (now constructor).
   - simpl. destruct (decide (n = x)). auto. constructor. apply Hp. subst. simpl. auto.  exact H.
   - simpl. constructor. apply Hp. subst. simpl. auto. exact H.
   - simpl. constructor. apply Hp. subst. simpl. auto. exact H. 
@@ -561,23 +546,23 @@ Qed.
 Inductive sts : proc -> proc -> Prop :=
 (*The axiomes*)
 (* Communication of channels output and input that have the same name *)
-| sts_com : forall {c v p2 g2}, (*Well_Defined_Input_in 0 (((c ! (cst v) • p1) + g1) ‖ ((c ? x • p2) + g2)) ->*)
-    sts ((c ! (cst v) • 𝟘) ‖ ((c ? x • p2) + g2)) (𝟘 ‖ (p2 ^ v))
+| sts_com : forall {c v p2 g2}, 
+    sts ((c ! v • 𝟘) ‖ ((c ? x • p2) + g2)) (𝟘 ‖ (p2 ^ v))
 (* Nothing more , something less *)
-| sts_tau : forall {p g}, (* Well_Defined_Input_in 0 (((t • p) + g)) -> *)
+| sts_tau : forall {p g}, 
     sts ((t • p) + g) p
 (* Resursion *)
-| sts_recursion : forall {x p}, (* Well_Defined_Input_in 0 (rec x • p) -> *)
+| sts_recursion : forall {x p}, 
     sts (rec x • p) (pr_subst x p (rec x • p))
 (*If Yes*)
-| sts_ifOne : forall {p q v v'}, v = v' -> (*Well_Defined_Input_in 0 (If (v == v') Then p Else q) ->*)
-    sts (If (v == v') Then p Else q) p
+| sts_ifOne : forall {p q E}, Eval_Eq E = Some true -> 
+    sts (If E Then p Else q) p
 (*If No*)
-| sts_ifZero : forall {p q v v'}, ~(v = v') -> (*Well_Defined_Input_in 0 (If (v == v') Then p Else q) ->*)
-    sts (If (v == v') Then p Else q) q
+| sts_ifZero : forall {p q E}, Eval_Eq E = Some false -> 
+    sts (If E Then p Else q) q
 
 (* The left parallele respect the Reduction *)
-| sts_par : forall {p1 p2 q}, (* Well_Defined_Input_in 0 q ->*)
+| sts_par : forall {p1 p2 q}, 
     sts p1 p2 ->
     sts (p1 ‖ q) (p2 ‖ q)
 
@@ -591,11 +576,11 @@ Inductive sts : proc -> proc -> Prop :=
 
 (* For the (STS-reduction), the reductible terms and reducted terms are pretty all the same, up to ≡* *)
 Lemma ReductionShape : forall P Q, sts P Q ->
-((exists c v P2 G2 S, ((P ≡* ((c ! (cst v) • 𝟘) ‖ ((c ? x • P2) + G2)) ‖ S)) /\ (Q ≡*((𝟘 ‖ (P2^v)) ‖ S)))
+((exists c v P2 G2 S, ((P ≡* ((c ! v • 𝟘) ‖ ((c ? x • P2) + G2)) ‖ S)) /\ (Q ≡*((𝟘 ‖ (P2^v)) ‖ S)))
 \/ (exists P1 G1 S, (P ≡* (((t • P1) + G1) ‖ S)) /\ (Q ≡* (P1 ‖ S)))
 \/ (exists n P1 S, (P ≡* ((rec n • P1) ‖ S)) /\ (Q ≡* (pr_subst n P1 (rec n • P1) ‖ S)))
-\/ (exists P1 P0 S v, (P ≡* ((If (v == v) Then P1 Else P0) ‖ S)) /\ (Q ≡* P1 ‖ S))
-\/ (exists P1 P0 S v v', (P ≡* ((If (v == v') Then P1 Else P0) ‖ S)) /\ (Q ≡* P0 ‖ S) /\ ~(v = v'))
+\/ (exists P1 P0 S E, (P ≡* ((If E Then P1 Else P0) ‖ S)) /\ (Q ≡* P1 ‖ S) /\ (Eval_Eq E = Some true))
+\/ (exists P1 P0 S E, (P ≡* ((If E Then P1 Else P0) ‖ S)) /\ (Q ≡* P0 ‖ S) /\ (Eval_Eq E = Some false))
 ).
 Proof.
 intros P Q Transition.
@@ -603,36 +588,44 @@ induction Transition.
   - left. exists c. exists v. exists p2. exists g2. exists (𝟘). split; apply cgr_par_nil_rev.
   - right. left. exists p. exists g0. exists 𝟘. split; apply cgr_par_nil_rev.
   - right. right. left. exists x. exists p. exists 𝟘. split; apply cgr_par_nil_rev.
-  - right. right. right. left. exists p. exists q. exists 𝟘. exists v. rewrite H.  split;apply cgr_par_nil_rev.
-  - right. right. right. right. exists p. exists q. exists 𝟘. exists v. exists v'. split. apply cgr_par_nil_rev.
-    split. apply cgr_par_nil_rev. auto.
-  - destruct IHTransition as [IH|[IH|[IH|[IH |IH]]]];  decompose record IH. 
-    * left. exists x. exists x0. exists x1. exists x2. exists (x3 ‖ q). split.
+  - right. right. right. left. exists p. exists q. exists 𝟘. exists E. split. apply cgr_par_nil_rev.
+    split. apply cgr_par_nil_rev. assumption.
+  - right. right. right. right. exists p. exists q. exists 𝟘. exists E. split. apply cgr_par_nil_rev.
+    split. apply cgr_par_nil_rev. assumption.
+  - destruct IHTransition as [IH|[IH|[IH|[IH |IH]]]]. 
+    * decompose record IH. left. exists x. exists x0. exists x1. exists x2. exists (x3 ‖ q). split.
         ** apply transitivity with ((((x ! x0 • 𝟘) ‖ ((x ? l • x1) + x2)) ‖ x3) ‖ q). apply cgr_par. auto. apply cgr_par_assoc.
         ** apply transitivity with (((𝟘 ‖ x1^x0) ‖ x3) ‖ q). apply cgr_par. auto.  apply cgr_par_assoc. 
-    * right. left. exists x. exists x0. exists (x1 ‖ q). split.
+    * decompose record IH. right. left. exists x. exists x0. exists (x1 ‖ q). split.
         ** apply transitivity with (((t • x + x0) ‖ x1) ‖ q). apply cgr_par. auto. apply cgr_par_assoc.
         ** apply transitivity with (x ‖ (x1) ‖ q). apply cgr_par. auto. apply cgr_par_assoc.
-    * right. right. left. exists x. exists x0. exists (x1 ‖ q). split. 
+    * decompose record IH. right. right. left. exists x. exists x0. exists (x1 ‖ q). split. 
         ** apply transitivity with ((rec x • x0 ‖ x1) ‖ q). apply cgr_par. assumption. apply cgr_par_assoc.
         ** apply transitivity with ((pr_subst x x0 (rec x • x0) ‖ x1) ‖ q). apply cgr_par. assumption. apply cgr_par_assoc.
-    * right. right. right. left. exists x. exists x0. exists (x1 ‖ q). exists x2. split.
-        ** apply transitivity with (((If (x2 == x2) Then x Else x0) ‖ x1) ‖ q). apply cgr_par. assumption. apply cgr_par_assoc.
-        ** apply transitivity with ((x ‖ x1) ‖ q). apply cgr_par. assumption. apply cgr_par_assoc.
-    * right. right. right. right. exists x. exists x0. exists (x1 ‖ q). exists x2. exists x3. split.
-        ** apply transitivity with (((If (x2 == x3) Then x Else x0) ‖ x1) ‖ q). apply cgr_par. assumption. apply cgr_par_assoc.
-        ** split. apply transitivity with ((x0 ‖ x1) ‖ q). apply cgr_par. assumption. apply cgr_par_assoc. auto.
-  - destruct IHTransition as [IH|[IH|[IH|[IH |IH]]]]; decompose record IH. 
-    * left. exists x. exists x0. exists x1. exists x2. exists x3.  split. apply cgr_trans with p2. exact H. exact H2.
+    * destruct IH. destruct H. destruct H. destruct H. destruct H. destruct H0.
+      right. right. right. left. exists x. exists x0. exists (x1 ‖ q). exists x2. split.
+        ** apply transitivity with (((If x2 Then x Else x0) ‖ x1) ‖ q). apply cgr_par. assumption. apply cgr_par_assoc.
+        ** split. apply transitivity with ((x ‖ x1) ‖ q). apply cgr_par. assumption. apply cgr_par_assoc. assumption.
+    * destruct IH. destruct H. destruct H. destruct H. destruct H. destruct H0.
+      right. right. right. right. exists x. exists x0. exists (x1 ‖ q). exists x2. split.
+        ** apply transitivity with (((If x2 Then x Else x0) ‖ x1) ‖ q). apply cgr_par. assumption. apply cgr_par_assoc.
+        ** split. apply transitivity with ((x0 ‖ x1) ‖ q). apply cgr_par. assumption. apply cgr_par_assoc. assumption.
+  - destruct IHTransition as [IH|[IH|[IH|[IH |IH]]]].  
+    * decompose record IH.
+      left. exists x. exists x0. exists x1. exists x2. exists x3.  split. apply cgr_trans with p2. exact H. exact H2.
       apply cgr_trans with q2. apply cgr_symm. exact H0. exact H3.
-    * right. left. exists x. exists x0. exists x1. split. apply cgr_trans with p2. exact H. exact H2. apply cgr_trans with q2.
+    * decompose record IH.
+      right. left. exists x. exists x0. exists x1. split. apply cgr_trans with p2. exact H. exact H2. apply cgr_trans with q2.
       apply cgr_symm. apply H0. apply H3.
-    * right. right. left. exists x. exists x0. exists x1. split. apply cgr_trans with p2. exact H. exact H2. apply cgr_trans with q2.
+    * decompose record IH. 
+      right. right. left. exists x. exists x0. exists x1. split. apply cgr_trans with p2. exact H. exact H2. apply cgr_trans with q2.
       apply cgr_symm. apply H0. apply H3.
-    * right. right. right. left. exists x. exists x0. exists x1. exists x2. split. apply cgr_trans with p2. exact H. exact H1. apply cgr_trans with q2.
-      apply cgr_symm. apply H0. apply H3.
-    * right. right. right. right. exists x. exists x0. exists x1. exists x2. exists x3. split. apply cgr_trans with p2. exact H. exact H2. split. apply cgr_trans with q2.
-      apply cgr_symm. apply H0. apply H1. auto.
+    * destruct IH. destruct H1. destruct H1. destruct H1. destruct H1. destruct H2.
+      right. right. right. left. exists x. exists x0. exists x1. exists x2. split. apply cgr_trans with p2. exact H. exact H1. split. apply cgr_trans with q2.
+      apply cgr_symm. apply H0. assumption. assumption.
+    * destruct IH. destruct H1. destruct H1. destruct H1. destruct H1. destruct H2.
+      right. right. right. right. exists x. exists x0. exists x1. exists x2. split. apply cgr_trans with p2. assumption. assumption. split. apply cgr_trans with q2.
+      apply cgr_symm. apply H0. assumption. assumption.
 Qed.
 
 (* For the (LTS-transition), the transitable terms and transitted terms, that performs a INPUT,
@@ -817,10 +810,10 @@ Proof.
     + intros. dependent destruction l. exists (p^v). split. apply lts_input.
       apply Congruence_Respects_Substitution. constructor. apply H.
     + intros. dependent destruction l.
-      -- destruct (IHcgr_step p2 (ActOut (c ⋉ (cst v)))).  exact l1. destruct H0. exists (x ‖ q2).
+      -- destruct (IHcgr_step p2 (ActOut (c ⋉ v))).  exact l1. destruct H0. exists (x ‖ q2).
           split. eapply lts_comL. exact H0. assumption.
           apply cgr_fullpar. assumption. reflexivity.
-      -- destruct (IHcgr_step q2 (ActIn (c ⋉ (cst v)))). assumption. destruct H0. exists (x ‖ p2).
+      -- destruct (IHcgr_step q2 (ActIn (c ⋉ v))). assumption. destruct H0. exists (x ‖ p2).
           split.  eapply lts_comR. exact l1. assumption.
           apply cgr_fullpar. assumption. reflexivity.
       -- destruct (IHcgr_step p2 α). assumption. destruct H0. eexists.
@@ -830,12 +823,11 @@ Proof.
           assumption. apply cgr_par.
           constructor. assumption.
     + intros. dependent destruction l.
-      -- eexists. split. instantiate (1:= p). apply lts_ifOne. reflexivity. 
-         constructor. reflexivity.
+      -- eexists. split. instantiate (1:= p). apply lts_ifOne. assumption. reflexivity. 
       -- eexists. split. instantiate (1:= q). apply lts_ifZero. assumption.
          constructor. assumption.
     + intros. dependent destruction l.
-      -- eexists. split. instantiate (1:= p). apply lts_ifOne. auto. 
+      -- eexists. split. instantiate (1:= p). apply lts_ifOne. assumption.
          constructor. assumption.
       -- eexists. split. instantiate (1:= q). apply lts_ifZero. assumption. 
          constructor. reflexivity.
@@ -852,18 +844,19 @@ Qed.
 Lemma Reduction_Implies_TausAndCong : forall P Q, (sts P Q) -> (lts_then_sc P τ Q).
 Proof. 
 intros P Q Reduction. 
-assert ((exists c v P2 G2 S, ((P ≡* ((c ! (cst v) • 𝟘) ‖ ((c ? x • P2) + G2)) ‖ S)) /\ (Q ≡*((𝟘 ‖ (P2^v)) ‖ S)))
+assert ((exists c v P2 G2 S, ((P ≡* ((c ! v • 𝟘) ‖ ((c ? x • P2) + G2)) ‖ S)) /\ (Q ≡*((𝟘 ‖ (P2^v)) ‖ S)))
 \/ (exists P1 G1 S, (P ≡* (((t • P1) + G1) ‖ S)) /\ (Q ≡* (P1 ‖ S)))
 \/ (exists n P1 S, (P ≡* ((rec n • P1) ‖ S)) /\ (Q ≡* (pr_subst n P1 (rec n • P1) ‖ S)))
-\/ (exists P1 P0 S v, (P ≡* ((If (v == v) Then P1 Else P0) ‖ S)) /\ (Q ≡* P1 ‖ S))
-\/ (exists P1 P0 S v v', (P ≡* ((If (v == v') Then P1 Else P0) ‖ S)) /\ (Q ≡* P0 ‖ S) /\ ~(v = v'))
+\/ (exists P1 P0 S E, (P ≡* ((If E Then P1 Else P0) ‖ S)) /\ (Q ≡* P1 ‖ S) /\ (Eval_Eq E = Some true))
+\/ (exists P1 P0 S E, (P ≡* ((If E Then P1 Else P0) ‖ S)) /\ (Q ≡* P0 ‖ S) /\ (Eval_Eq E = Some false))
 ). 
 apply ReductionShape. exact Reduction.
-destruct H as [IH|[IH|[IH|[IH |IH]]]];  decompose record IH. 
+destruct H as [IH|[IH|[IH|[IH |IH]]]]. 
 
 (*First case τ by communication *)
 
-- assert (lts ((x ! x0 • 𝟘) ‖ ((x ? l • x1) + x2) ‖ x3) τ (𝟘 ‖ (x1^x0) ‖ x3)).
+- decompose record IH.
+  assert (lts ((x ! x0 • 𝟘) ‖ ((x ? l • x1) + x2) ‖ x3) τ (𝟘 ‖ (x1^x0) ‖ x3)).
   * apply lts_parL.   
     eapply lts_comL. instantiate (2:= x). instantiate (1:= x0).
     apply lts_output. apply lts_choiceL. apply lts_input.
@@ -873,7 +866,8 @@ destruct H as [IH|[IH|[IH|[IH |IH]]]];  decompose record IH.
 
 (*Second case τ by Tau Action *)
 
-- assert (lts ((t • x + x0) ‖ x1) τ (x ‖ x1)). constructor.
+- decompose record IH.
+  assert (lts ((t • x + x0) ‖ x1) τ (x ‖ x1)). constructor.
   apply lts_choiceL. apply lts_tau.
   assert (sc_then_lts P τ (x ‖ x1)). exists ((t • x + x0) ‖ x1). split. assumption. apply lts_parL.
   apply lts_choiceL. apply lts_tau.
@@ -882,7 +876,8 @@ destruct H as [IH|[IH|[IH|[IH |IH]]]];  decompose record IH.
 
 (*Third case τ by recursion *)
 
-- assert (lts (rec x • x0 ‖ x1) τ (pr_subst x x0 (rec x • x0) ‖ x1)). 
+- decompose record IH.
+  assert (lts (rec x • x0 ‖ x1) τ (pr_subst x x0 (rec x • x0) ‖ x1)). 
   constructor. apply lts_recursion. assert (sc_then_lts P τ ((pr_subst x x0 (rec x • x0) ‖ x1))). 
   exists (rec x • x0 ‖ x1). split. assumption. assumption. assert (lts_then_sc P τ (pr_subst x x0 (rec x • x0) ‖ x1)). 
   apply Congruence_Respects_Transition. assumption. destruct H3. destruct H3. 
@@ -891,22 +886,24 @@ destruct H as [IH|[IH|[IH|[IH |IH]]]];  decompose record IH.
 
 (*Fourth case τ by If ONE*)
 
-- assert (lts ((If x2 == x2 Then x Else x0) ‖ x1) τ (x ‖ x1)). constructor. apply lts_ifOne. auto.
-  assert (sc_then_lts P τ (x ‖ x1)). exists ((If x2 == x2 Then x Else x0) ‖ x1). split. assumption.
-  constructor. constructor. auto. 
+- destruct IH. destruct H. destruct H. destruct H. destruct H. destruct H0. 
+  assert (lts ((If x2 Then x Else x0) ‖ x1) τ (x ‖ x1)). constructor. apply lts_ifOne. assumption.
+  assert (sc_then_lts P τ (x ‖ x1)). exists ((If x2 Then x Else x0) ‖ x1). split. assumption.
+  constructor. constructor. assumption. 
   assert (lts_then_sc P τ (x ‖ x1)). apply Congruence_Respects_Transition. 
-  exists ((If x2 == x2 Then x Else x0) ‖ x1). split. assumption. assumption. destruct H3. destruct H3.
+  exists ((If x2 Then x Else x0) ‖ x1). split. assumption. assumption. destruct H4. destruct H4.
   exists x3. split. assumption. apply transitivity with (x ‖ x1). assumption. 
-  symmetry. exact H1. 
+  symmetry. assumption.
 
 (*Fifth case τ by If ZERO*)
 
-- assert (lts ((If x2 == x3 Then x Else x0) ‖ x1) τ (x0 ‖ x1)). constructor. apply lts_ifZero. assumption.
-  assert (sc_then_lts P τ (x0 ‖ x1)). exists ((If x2 == x3 Then x Else x0) ‖ x1). split. assumption.
+- destruct IH. destruct H. destruct H. destruct H. destruct H. destruct H0. 
+  assert (lts ((If x2 Then x Else x0) ‖ x1) τ (x0 ‖ x1)). constructor. apply lts_ifZero. assumption.
+  assert (sc_then_lts P τ (x0 ‖ x1)). exists ((If x2 Then x Else x0) ‖ x1). split. assumption.
   apply lts_parL. apply lts_ifZero. assumption.
   assert (lts_then_sc P τ (x0 ‖ x1)). apply Congruence_Respects_Transition. 
-  exists ((If x2 == x3 Then x Else x0) ‖ x1). split.  assumption. assumption. destruct H4. destruct H4.
-  exists x4. split. assumption. apply transitivity with (x0 ‖ x1). assumption.
+  exists ((If x2 Then x Else x0) ‖ x1). split.  assumption. assumption. destruct H4. destruct H4.
+  exists x3. split. assumption. apply transitivity with (x0 ‖ x1). assumption.
   symmetry. assumption. 
 Qed.
 
@@ -1009,10 +1006,14 @@ Qed.
 (* Definition for Well Abstracted bvariable *)
 Inductive Well_Defined_Data : nat -> Data -> Prop :=
 | bvar_is_defined_up_to_k: forall k x, (x < k) -> Well_Defined_Data k (bvar x)
-| cst_is_always_defined : forall k x, Well_Defined_Data k (cst x).
+| cst_is_always_defined : forall k v, Well_Defined_Data k (cst v).
 
 Inductive Well_Defined_Condition : nat -> Equation Data -> Prop :=
-| equationOnValueXX : forall k x y, Well_Defined_Data k x -> Well_Defined_Data k y -> Well_Defined_Condition k (x == y).
+| tt_is_WD : forall k, Well_Defined_Condition k tt
+| ff_is_WD : forall k, Well_Defined_Condition k ff
+| Inequality_is_WD : forall k x y, Well_Defined_Data k x -> Well_Defined_Data k y -> Well_Defined_Condition k (x ⩽ y)
+| Or_is_WD : forall k e e', Well_Defined_Condition k e -> Well_Defined_Condition k e' -> Well_Defined_Condition k (e ∨ e')
+| Not_is_WD : forall k e, Well_Defined_Condition k e -> Well_Defined_Condition k (non e).
 
 Inductive Well_Defined_Input_in : nat -> proc -> Prop :=
 | WD_par : forall k p1 p2, Well_Defined_Input_in k p1 -> Well_Defined_Input_in k p2 
@@ -1041,11 +1042,16 @@ Qed.
 
 Lemma Inequation_k_equation : forall k c, Well_Defined_Condition k c -> Well_Defined_Condition (S k) c.
 Proof.
-intros. dependent destruction c. destruct d; destruct d0.
-- constructor; constructor.
-- dependent destruction H. constructor. constructor. apply Inequation_k_data. assumption.
-- dependent destruction H. constructor. apply Inequation_k_data. assumption. constructor. 
-- dependent destruction H. constructor; apply Inequation_k_data; assumption.
+intros. dependent induction c.
+* constructor.
+* constructor.
+* destruct a; destruct a0.
+  - constructor; constructor.
+  - dependent destruction H. constructor. constructor. apply Inequation_k_data. assumption.
+  - dependent destruction H. constructor. apply Inequation_k_data. assumption. constructor. 
+  - dependent destruction H. constructor; apply Inequation_k_data; assumption.
+* dependent destruction H. constructor. apply IHc1. assumption. apply IHc2. assumption.
+* dependent destruction H. constructor. apply IHc. assumption.
 Qed.
 
 Lemma Inequation_k_proc : forall k p, Well_Defined_Input_in k p -> Well_Defined_Input_in (S k) p.
@@ -1118,7 +1124,7 @@ Proof.
 intros. revert H. revert v. revert k. dependent induction d.
 * intros. simpl. constructor.
 * intros. simpl. destruct (decide (n = k )).
-  - constructor.
+  - constructor. 
   - dependent destruction H. constructor. apply NotK; assumption.
 Qed.
 
@@ -1126,7 +1132,10 @@ Lemma ForEquation : forall k v e, Well_Defined_Condition (S k) e
                 -> Well_Defined_Condition k (subst_in_Equation k (cst v) e).
 Proof.
 intros. revert H. revert v. revert k. 
-- dependent destruction e. dependent induction d; dependent induction d0.
+- dependent induction e. 
+-- intros. simpl. constructor.
+-- intros. simpl. constructor.
+-- dependent induction a; dependent induction a0.
   * intros. simpl. constructor; constructor.
   * intros. simpl. destruct (decide (n = k)).
     ** constructor; constructor.
@@ -1138,6 +1147,8 @@ intros. revert H. revert v. revert k.
     apply NotK; assumption.
     ** destruct (decide (n0 = k)); try constructor. dependent destruction H. dependent destruction H0. 
     apply NotK; assumption.
+-- intros. dependent destruction H. simpl. constructor. apply IHe1. assumption. apply IHe2. assumption.
+-- intros. dependent destruction H. simpl. constructor. apply IHe. assumption.
 Qed.
 
 Lemma ForSTS : forall k p v, Well_Defined_Input_in (S k) p -> Well_Defined_Input_in k (subst_in_proc k (cst v) p).
@@ -1207,18 +1218,26 @@ destruct p'.
       assumption. assumption.
 Qed.
 
-Lemma RecursionOverReduction_is_WD : forall k x p, Well_Defined_Input_in k (rec x • p) -> Well_Defined_Input_in k (pr_subst x p (rec x • p)).
+Lemma RecursionOverReduction_is_WD : forall k x p, Well_Defined_Input_in k (rec x • p) 
+          -> Well_Defined_Input_in k (pr_subst x p (rec x • p)).
 Proof.
 intros. apply ForRecursionSanity. dependent destruction H. assumption. assumption.
 Qed.
 
+Lemma Well_Def_Data_Is_a_value : forall d, Well_Defined_Data 0 d <-> exists v, d = cst v.
+Proof.
+intros. split. 
+- intro. dependent destruction H. exfalso. dependent induction H. exists v. reflexivity.
+- intros. destruct H. subst. constructor.
+Qed.
 
 Lemma STS_Respects_WD : forall p q, Well_Defined_Input_in 0 p -> sts p q -> Well_Defined_Input_in 0 q.
 Proof.
 intros. revert H. rename H0 into Reduction. dependent induction Reduction.
 * intros. constructor.
   - constructor.
-  - dependent destruction H. dependent destruction H0. dependent destruction H0_. apply ForSTS. assumption. 
+  - dependent destruction H. dependent destruction H0. dependent destruction H0_. 
+    dependent destruction H. apply Well_Def_Data_Is_a_value in H. destruct H. subst.  apply ForSTS. assumption. 
 * intros. dependent destruction H. dependent destruction H. assumption.
 * intros. dependent destruction H. apply RecursionOverReduction_is_WD. constructor. assumption.
 * intros. dependent destruction H0. assumption.
@@ -1228,42 +1247,64 @@ intros. revert H. rename H0 into Reduction. dependent induction Reduction.
   assumption. assumption. assumption.
 Qed.
 
-Lemma LTS_Respects_WD : forall p q α, Well_Defined_Input_in 0 p -> lts p α q ->  Well_Defined_Input_in 0 q.
+Inductive Well_Defined_Action: (Act TypeOfActions) -> Prop :=
+| ActionOuput_with_value_is_always_defined : forall c v, Well_Defined_Action (ActOut  (c ⋉ (cst v)))
+| ActionInput_with_value_is_always_defined : forall c v, Well_Defined_Action (ActIn  (c ⋉ (cst v)))
+| Tau_is_always_defined : Well_Defined_Action (τ).
+
+Lemma Output_are_good : forall p1 p2 c d, Well_Defined_Input_in 0 p1 -> lts p1 (ActOut (c ⋉ d)) p2 
+      -> exists v, d = cst v.
 Proof.
-intros. revert H. rename H0 into Transition. dependent induction Transition.
-* intros. apply ForSTS. dependent destruction H. assumption.
+intros. dependent induction H0. dependent destruction H. apply Well_Def_Data_Is_a_value in H. destruct H.
+subst. exists x. reflexivity.
+- dependent destruction H. eapply IHlts with c. assumption. reflexivity.
+- dependent destruction H. eapply IHlts with c. assumption. reflexivity.
+- dependent destruction H. eapply IHlts with c. assumption. reflexivity.
+- dependent destruction H. eapply IHlts with c. assumption. reflexivity.
+Qed.
+
+Lemma LTS_Respects_WD : forall p q α, Well_Defined_Input_in 0 p -> Well_Defined_Action α -> lts p α q 
+            ->  Well_Defined_Input_in 0 q.
+Proof.
+intros. revert H. revert H0. rename H1 into Transition. dependent induction Transition.
+* intros. dependent destruction H0.  apply ForSTS. dependent destruction H. assumption.
 * intros. constructor.
 * intros. dependent destruction H. assumption.
 * intros. apply ForRecursionSanity. dependent destruction H. assumption. assumption.
-* intros. dependent destruction H0. assumption.
-* intros. dependent destruction H0. assumption.
+* intros. dependent destruction H1. assumption.
+* intros. dependent destruction H1. assumption.
 * intros. dependent destruction H. constructor. 
-  ** apply IHTransition1. assumption.
-  ** apply IHTransition2. assumption.
+  ** apply IHTransition1. assert (exists v', v = cst v'). eapply Output_are_good. exact H.
+     exact Transition1. destruct H2. subst. constructor. assumption.
+  ** apply IHTransition2. assert (exists v', v = cst v'). eapply Output_are_good. exact H.
+     exact Transition1. destruct H2. subst. constructor. assumption.
 * intros. dependent destruction H. constructor.
-  ** apply IHTransition2. assumption.
-  ** apply IHTransition1. assumption.
-* intros. dependent destruction H. constructor. apply IHTransition. assumption. assumption.
-* intros. dependent destruction H. constructor. assumption. apply IHTransition. assumption.
-* intros. dependent destruction H. apply IHTransition. assumption.
-* intros. dependent destruction H. apply IHTransition. assumption.
+  ** apply IHTransition2. assert (exists v', v = cst v'). eapply Output_are_good. exact H1.
+     exact Transition1. destruct H2. subst. constructor. assumption.
+  ** apply IHTransition1. assert (exists v', v = cst v'). eapply Output_are_good. exact H1.
+     exact Transition1. destruct H2. subst. constructor. assumption.
+* intros. dependent destruction H. constructor. apply IHTransition. assumption. assumption. assumption.
+* intros. dependent destruction H. constructor. assumption. apply IHTransition. assumption. assumption.
+* intros. dependent destruction H. apply IHTransition. assumption. assumption.
+* intros. dependent destruction H. apply IHTransition. assumption. assumption.
 Qed.
+
 
 (* Lemma to simplify the Data in Value for a transition *)
-Lemma OutputWithValue : forall p q a, lts p (ActOut a) q -> exists c v, a = c ⋉ (cst v).
+Lemma OutputWithValue : forall p q a, lts p (ActOut a) q -> exists c d, a = c ⋉ d.
 Proof.
 intros. dependent destruction a. dependent induction H.
-- exists c. exists v. reflexivity.
+- exists c. exists d. reflexivity.
 - destruct (IHlts c d). reflexivity. destruct H0. dependent destruction H0. exists x. exists x0. reflexivity.
 - destruct (IHlts c d). reflexivity. destruct H0. dependent destruction H0. exists x. exists x0. reflexivity.
 - destruct (IHlts c d). reflexivity. destruct H0. dependent destruction H0. exists x. exists x0. reflexivity.
 - destruct (IHlts c d). reflexivity. destruct H0. dependent destruction H0. exists x. exists x0. reflexivity.
 Qed.
 
-Lemma InputWithValue : forall p q a, lts p (ActIn a) q -> exists c v, a = c ⋉ (cst v).
+Lemma InputWithValue : forall p q a, lts p (ActIn a) q -> exists c v, a = c ⋉ v.
 Proof.
 intros. dependent destruction a. dependent induction H.
-- exists c. exists v. reflexivity.
+- exists c. exists d. reflexivity.
 - destruct (IHlts c d). reflexivity. destruct H0. dependent destruction H0. exists x. exists x0. reflexivity.
 - destruct (IHlts c d). reflexivity. destruct H0. dependent destruction H0. exists x. exists x0. reflexivity.
 - destruct (IHlts c d). reflexivity. destruct H0. dependent destruction H0. exists x. exists x0. reflexivity.
@@ -1275,7 +1316,7 @@ Qed.
 
 Lemma OBA_with_FB_First_Axiom : forall p q r a α,
   lts p (ActOut a) q -> lts q α r ->
-  (exists r', lts p α r' /\ lts_then_sc r' (ActOut a) r).
+  (exists r', lts p α r' /\ lts_then_sc r' (ActOut a) r). (* output-commutativity *)
 Proof.
 intros. assert (lts p (ActOut a) q). assumption. apply OutputWithValue in H1.
 decompose record H1. subst. eapply TransitionShapeForOutputSimplified in H.
@@ -1283,17 +1324,17 @@ eapply lts_parR in H0. instantiate (1 := (x ! x0 • 𝟘)) in H0.
 edestruct (Congruence_Respects_Transition p ((x ! x0 • 𝟘) ‖ r) α).
 exists ((x ! x0 • 𝟘) ‖ q). split; assumption. destruct H2.
 assert (lts ((x ! x0 • 𝟘) ‖ r) (ActOut (x ⋉ x0)) (𝟘 ‖ r)). constructor. constructor.
-edestruct (Congruence_Respects_Transition x1 (𝟘 ‖ r) (ActOut (x ⋉ (cst x0)))).
+edestruct (Congruence_Respects_Transition x1 (𝟘 ‖ r) (ActOut (x ⋉ x0))).
 exists ((x ! x0 • 𝟘) ‖ r). split ; assumption. destruct H5.
 assert (x2 ≡* r). eauto with cgr.
 exists x1. split. assumption. exists x2. split; assumption.
 Qed.
 
-Lemma OBA_with_FB_Second_Axiom : forall p q1 q2 a μ,
+Lemma OBA_with_FB_Second_Axiom : forall p q1 q2 a μ, 
   μ ≠ (ActOut a) ->
   lts p (ActOut a) q1 ->
   lts p (ActExt μ) q2 ->
-  ∃ r : proc, lts q1 (ActExt μ) r ∧ lts_then_sc q2 (ActOut a) r.
+  ∃ r : proc, lts q1 (ActExt μ) r ∧ lts_then_sc q2 (ActOut a) r. (* output-confluence  *)
 Proof.
 intros. assert (lts p (ActOut a) q1). assumption. apply OutputWithValue in H2.
 decompose record H2. subst. rename x into c. rename x0 into v.
@@ -1303,14 +1344,14 @@ exists p. split. symmetry. assumption. assumption.
 destruct H3. inversion H3; subst.
 inversion H9. subst. now destruct H. 
 exists q3. split. assumption.
-assert (lts ((c ! v • 𝟘) ‖ q3) (ActOut (c ⋉ (cst v))) (𝟘 ‖ q3)). constructor. constructor.
-edestruct (Congruence_Respects_Transition q2 (𝟘 ‖ q3) (ActOut (c ⋉ (cst v)))).
+assert (lts ((c ! v • 𝟘) ‖ q3) (ActOut (c ⋉ v)) (𝟘 ‖ q3)). constructor. constructor.
+edestruct (Congruence_Respects_Transition q2 (𝟘 ‖ q3) (ActOut (c ⋉ v))).
 exists ((c ! v • 𝟘) ‖ q3). split. eauto with cgr. assumption. destruct H6. exists x. split. assumption.
 eauto with cgr.
 Qed.
 
-Lemma OBA_with_FB_Third_Axiom : forall p1 p2 p3 a,
-            lts p1 (ActOut a) p2 → lts p1 (ActOut a) p3 -> p2 ≡* p3.
+Lemma OBA_with_FB_Third_Axiom : forall p1 p2 p3 a, 
+            lts p1 (ActOut a) p2 → lts p1 (ActOut a) p3 -> p2 ≡* p3. (* output-determinacy *)
 Proof.
 intros. assert (lts p1 (ActOut a) p2). assumption. apply OutputWithValue in H1.
 decompose record H1. subst. rename x into c. rename x0 into v.
@@ -1336,12 +1377,12 @@ revert H0. revert p3. dependent induction H.
 Qed.
 
 Lemma OBA_with_FB_Fourth_Axiom : forall p1 p2 p3 a, lts p1 (ActOut a) p2 -> lts p2 (ActIn a) p3 
-                              -> lts_then_sc p1 τ p3.
+                              -> lts_then_sc p1 τ p3. (* feedback *)
 Proof.
 intros. assert (lts p1 (ActOut a) p2). assumption. apply OutputWithValue in H1.
 decompose record H1. subst. rename x into c. rename x0 into v.
 eapply TransitionShapeForOutputSimplified in H.
-assert (lts (c ! v • 𝟘) (ActOut (c ⋉ (cst v))) 𝟘). constructor.
+assert (lts (c ! v • 𝟘) (ActOut (c ⋉ v)) 𝟘). constructor.
 assert (lts ((c ! v • 𝟘) ‖ p2) τ  (𝟘 ‖ p3)). econstructor; eassumption.
 edestruct (Congruence_Respects_Transition p1 (𝟘 ‖ p3) τ). exists ((c ! v • 𝟘) ‖ p2).
 split; assumption. destruct H4. exists x. split. assumption. eauto with cgr.
@@ -1349,7 +1390,7 @@ Qed.
 
 Lemma OBA_with_FB_Fifth_Axiom : forall p q1 q2 a,
   lts p (ActOut a) q1 -> lts p τ q2 ->
-  (∃ q : proc, lts q1 τ q /\ lts_then_sc q2 (ActOut a) q) \/ lts_then_sc q1 (ActIn a) q2.
+  (∃ q : proc, lts q1 τ q /\ lts_then_sc q2 (ActOut a) q) \/ lts_then_sc q1 (ActIn a) q2. (* output-tau  *)
 Proof.
 intros. assert (lts p (ActOut a) q1). assumption. apply OutputWithValue in H1.
 decompose record H1. subst. rename x into c. rename x0 into v.
@@ -1360,8 +1401,8 @@ destruct H2. dependent induction H2.
 - inversion H2_0.
 - inversion H2.
 - left. exists q0. split. assumption. 
-  assert (lts ((c ! v • 𝟘) ‖ q0) (ActOut (c ⋉ (cst v))) (𝟘 ‖ q0)). constructor. constructor.
-  edestruct (Congruence_Respects_Transition q2 (𝟘 ‖ q0) (ActOut (c ⋉ (cst v)))). exists ((c ! v • 𝟘) ‖ q0).
+  assert (lts ((c ! v • 𝟘) ‖ q0) (ActOut (c ⋉ v)) (𝟘 ‖ q0)). constructor. constructor.
+  edestruct (Congruence_Respects_Transition q2 (𝟘 ‖ q0) (ActOut (c ⋉ v))). exists ((c ! v • 𝟘) ‖ q0).
   split. eauto with cgr. assumption. destruct H5. exists x. split. assumption. eauto with cgr.
 Qed.
 
@@ -1377,24 +1418,584 @@ apply transitivity with ((c ! v • 𝟘) ‖ q1). assumption.
 apply transitivity with ((c ! v • 𝟘) ‖ q2). eauto with cgr. eauto with cgr.
 Qed. 
 
+Hypothesis channel_eq_dec : EqDecision Channel.
+#[global] Instance channel_eqdecision : EqDecision Channel. by exact channel_eq_dec. Defined.
+Hypothesis channel_is_countable : Countable Channel.
+#[global] Instance channel_countable : Countable Channel. by exact channel_is_countable. Defined.
+Hypothesis value_eq_dec : EqDecision Value.
+#[global] Instance value_eqdecision : EqDecision Value. by exact value_eq_dec. Defined.
+Hypothesis value_is_countable : Countable Value.
+#[global] Instance value_countable : Countable Value. by exact value_is_countable. Defined.
+
+Lemma Data_dec : forall (x y : Data) , {x = y} + {x <> y}.
+Proof.
+decide equality. 
+* destruct (decide(v = v0)). left. assumption. right. assumption.
+* destruct (decide (n = n0)). left. assumption. right. assumption.
+Qed.
+
+#[global] Instance data_eqdecision : EqDecision Data. by exact Data_dec . Defined.
+
+Definition encode_data (D : Data) : gen_tree (nat + Value) :=
+match D with
+  | cst v => GenLeaf (inr v)
+  | bvar i => GenLeaf (inl i)
+end.
+
+Definition decode_data (tree : gen_tree (nat + Value)) : Data :=
+match tree with
+  | GenLeaf (inr v) => cst v
+  | GenLeaf (inl i) => bvar i
+  | _ => bvar 0
+end. 
+
+Lemma encode_decide_datas d : decode_data (encode_data d) = d.
+Proof. case d. 
+* intros. simpl. reflexivity.
+* intros. simpl. reflexivity.
+Qed.
+
+#[global] Instance data_countable : Countable Data.
+Proof.
+  refine (inj_countable' encode_data decode_data _).
+  apply encode_decide_datas.
+Qed.
+
+
+Fixpoint encode_equation (E : Equation Data) : gen_tree (nat + Data) :=
+match E with
+  | tt => GenLeaf (inl 1)
+  | ff => GenLeaf (inl 0)
+  | D1 ⩽ D2 => GenNode 2 [GenLeaf (inr D1) ; GenLeaf (inr D2)]
+  | e1 ∨ e2 => GenNode 3 [encode_equation e1 ; encode_equation e2]
+  | non e => GenNode 4 [encode_equation e] 
+end.
+
+Fixpoint decode_equation (tree : gen_tree (nat + Data)) : Equation Data :=
+match tree with
+  | GenLeaf (inl 1) => tt
+  | GenLeaf (inl 0) => ff
+  | GenNode 2 [GenLeaf (inr d); GenLeaf (inr d')] => d ⩽ d'
+  | GenNode 3 [p ; q] => (decode_equation p) ∨ (decode_equation q)
+  | GenNode 4 [t'] => non (decode_equation t')
+  | _ => ff
+end. 
+
+Lemma Equation_dec : forall (x y : Equation Data) , {x = y} + {x <> y}.
+Proof.
+decide equality. apply Data_dec. apply Data_dec.
+Qed.
+
+#[global] Instance equation_dec : EqDecision (Equation Data). exact Equation_dec. Defined.
+
+Lemma encode_decide_equations p : decode_equation (encode_equation p) = p.
+Proof. 
+induction p.
+* simpl. reflexivity.
+* simpl. reflexivity.
+* simpl. reflexivity.
+* simpl. rewrite IHp1. rewrite IHp2. reflexivity.
+* simpl. rewrite IHp. reflexivity.
+Qed.
+
+#[global] Instance equation_countable : Countable (Equation Data).
+Proof.
+  refine (inj_countable' encode_equation decode_equation _).
+  apply encode_decide_equations.
+Qed.
+
+Lemma TypeOfActions_dec : forall (x y : TypeOfActions) , {x = y} + {x <> y}.
+Proof.
+decide equality. 
+* destruct (decide(d = d0)). left. assumption. right. assumption.
+* destruct (decide (c = c0)). left. assumption. right. assumption.
+Qed.
+
+#[global] Instance TypeOfActions_eqdecision : EqDecision TypeOfActions. by exact TypeOfActions_dec . Defined.
+
+Fixpoint proc_dec (x y : proc) : { x = y } + { x <> y }
+with gproc_dec (x y : gproc) : { x = y } + { x <> y }.
+Proof.
+decide equality. 
+* destruct (decide(n = n0));eauto.
+* destruct (decide(n = n0));eauto.
+* destruct (decide(e = e0));eauto. 
+* destruct (decide(d = d0));eauto.
+* destruct (decide(c = c0));eauto.
+* decide equality. destruct (decide(c = c0));eauto.
+Qed.
+
+#[global] Instance proc_eqdecision : EqDecision proc. by exact proc_dec. Defined.
+
+Definition encode_TypeOfActions (a : TypeOfActions) : gen_tree (nat + (Channel + Data)) :=
+match a with
+  | act c v => GenNode 0 [GenLeaf (inr (inl c)) ; GenLeaf (inr (inr v))]
+end.
+
+Definition decode_TypeOfActions (tree :gen_tree (nat + (Channel + Data))) : option TypeOfActions :=
+match tree with
+  | GenNode 0 [GenLeaf (inr (inl c)); GenLeaf (inr (inr v))] => Some (act c v)
+  | _ => None
+end. 
+
+Lemma encode_decide_TypeOfActions p : decode_TypeOfActions (encode_TypeOfActions  p) = Some p.
+Proof. 
+induction p. 
+* simpl. reflexivity.
+Qed.
+
+#[global] Instance TypeOfActions_countable : Countable TypeOfActions.
+Proof.
+  eexists. intros. admit.
+Admitted.
+
+Fixpoint encode_proc (p: proc) : gen_tree (nat + (((Equation Data ) + TypeOfActions) + Channel)) :=
+  match p with
+  | p ‖ q  => GenNode 0 [encode_proc p; encode_proc q]
+  | c ! v • 𝟘  => GenLeaf (inr $ inl $ inr $ (c ⋉ v))
+  | pr_var i => GenNode 2 [GenLeaf $ inl i]
+  | rec x • P => GenNode 3 [GenLeaf $ inl x; encode_proc P]
+  | If C Then A Else B => GenNode 4 [GenLeaf (inr ( inl (inl C))) ; encode_proc A; encode_proc B]
+  | g gp => GenNode 1 [encode_gproc gp]
+  end
+with
+encode_gproc (gp: gproc) : gen_tree (nat + (((Equation Data ) + TypeOfActions) + Channel)) :=
+  match gp with
+  | ① => GenNode 1 []
+  | 𝟘 => GenNode 0 []
+  | c ? x • p => GenNode 2 [GenLeaf (inr $ inr c); encode_proc p]
+  | t • p => GenNode 3 [encode_proc p]
+  | gp + gq => GenNode 4 [encode_gproc gp; encode_gproc gq]
+  end.
+  
+Definition Channel_of (a : TypeOfActions) : Channel := 
+match a with 
+| act c d => c
+end.
+
+Definition Data_of (a : TypeOfActions) : Data := 
+match a with 
+| act c d => d
+end.
+
+Fixpoint decode_proc (t': gen_tree (nat + (((Equation Data ) + TypeOfActions) + Channel))) : proc :=
+  match t' with
+  | GenNode 0 [ep; eq] => (decode_proc ep) ‖ (decode_proc eq)
+  | GenLeaf (inr ( inl (inr a))) => (Channel_of a) ! (Data_of a) • 𝟘
+  | GenNode 2 [GenLeaf (inl i)] => pr_var i
+  | GenNode 3 [GenLeaf (inl i); egq] => rec i • (decode_proc egq)
+  | GenNode 4 [GenLeaf (inr ( inl (inl C))); A; B] => If C Then (decode_proc A) Else (decode_proc B)
+  | GenNode 1 [egp] => g (decode_gproc egp)
+  | _ => ① 
+  end
+with
+decode_gproc (t': gen_tree (nat + (((Equation Data ) + TypeOfActions) + Channel))): gproc :=
+  match t' with
+  | GenNode 1 [] => ①
+  | GenNode 0 [] => 𝟘
+  | GenNode 2 [GenLeaf (inr (inr c)); ep] => c ? x • (decode_proc ep)
+  | GenNode 3 [eq] => t • (decode_proc eq)
+  | GenNode 4 [egp; egq] => (decode_gproc egp) + (decode_gproc egq)
+  | _ => ① 
+  end.
+
+Lemma encode_decide_procs p : decode_proc (encode_proc p) = p
+with encode_decide_gprocs p : decode_gproc (encode_gproc p) = p.
+Proof. all: case p. 
+* intros. simpl. rewrite (encode_decide_procs p0). rewrite (encode_decide_procs p1). reflexivity.
+* intros. simpl. reflexivity.
+* intros. simpl. rewrite (encode_decide_procs p0). reflexivity.
+* intros. simpl. rewrite (encode_decide_procs p0). rewrite (encode_decide_procs p1). reflexivity.
+* intros. simpl. reflexivity.
+* intros. simpl. rewrite (encode_decide_gprocs g0). reflexivity.
+* intros. simpl. reflexivity. 
+* intros. simpl. reflexivity. 
+* intros. simpl. rewrite (encode_decide_procs p0). reflexivity.
+* intros. simpl. rewrite (encode_decide_procs p0). reflexivity.
+* intros. simpl. rewrite (encode_decide_gprocs g0). rewrite (encode_decide_gprocs g1). reflexivity.
+Qed.
+
+#[global] Instance proc_count : Countable proc.
+refine (inj_countable' encode_proc decode_proc _).
+  apply encode_decide_procs.
+Qed.
+#[global] Instance Singletons_of_TypeOfActions : SingletonMS TypeOfActions (gmultiset TypeOfActions) 
+:=gmultiset_singleton.
+#[global] Instance Singletons_of_proc : Singleton proc (gset proc) := gset_singleton.
+#[global] Instance Empty_of_proc : Empty (gset proc) := gset_empty.
+#[global] Instance Union_of_proc : Union (gset proc) := gset_union.
+#[global] Instance SemiSet_of_proc : SemiSet proc (gset proc) := gset_semi_set.
+
+(* Next Obligations *)
+Fixpoint moutputs_of p : gmultiset TypeOfActions := 
+match p with
+  | P ‖ Q => (moutputs_of P) ⊎ (moutputs_of Q)
+  | pr_var _ => ∅
+  | rec _ • _ => ∅
+  | If C Then P Else Q => ∅
+  | c ! v • 𝟘 => {[+ c ⋉ v +]}
+  | g _ => ∅
+end.  
+Definition outputs_of p := dom (moutputs_of p).
+
+Lemma mo_equiv_spec_step : forall {p q}, p ≡ q -> moutputs_of p = moutputs_of q.
+Proof. intros. dependent induction H; multiset_solver. Qed.
+
+Lemma mo_equiv_spec : forall {p q}, p ≡* q -> moutputs_of p = moutputs_of q.
+Proof.
+  intros p q hcgr.
+  induction hcgr. now eapply mo_equiv_spec_step.
+  etrans; eauto.
+Qed.
+
+Lemma mo_spec p a q : lts p (ActOut a) q -> moutputs_of p = {[+ a +]} ⊎ moutputs_of q.
+Proof.
+  intros l. assert (lts p (ActOut a) q). assumption. apply OutputWithValue in H.
+  decompose record H. subst. rename x into c. rename x0 into v.
+  eapply TransitionShapeForOutputSimplified, mo_equiv_spec in l. simpl in l. eauto.
+Qed.
+
+Lemma mo_spec_l e a :
+  a ∈ moutputs_of e -> {e' | lts e (ActExt $ ActOut a) e' /\ moutputs_of e' = moutputs_of e ∖ {[+ a +]}}.
+Proof.
+  intros mem.
+  dependent induction e.
+  + cbn in mem.
+    destruct (decide (a ∈ moutputs_of e1)).
+    destruct (IHe1 a e) as (e1' & lts__e1 & eq).
+    exists (pr_par e1' e2). repeat split; eauto with ccs.
+    multiset_solver.
+    destruct (decide (a ∈ moutputs_of e2)).
+    destruct (IHe2 a e) as (e2' & lts__e2 & eq).
+    exists (pr_par e1 e2'). repeat split; eauto with ccs.
+    multiset_solver.
+    contradict mem. intro mem. multiset_solver.
+    + exfalso. multiset_solver.
+    + exfalso. multiset_solver.
+    + exfalso. multiset_solver.
+  + exists (g 𝟘).
+    assert (a = c ⋉ d). multiset_solver. subst.
+    repeat split; eauto with ccs. multiset_solver.
+  + simpl in mem. exfalso. set_solver. 
+Qed.
+
+Lemma mo_spec_r e a :
+  {e' | lts e (ActExt $ ActOut a) e' /\ moutputs_of e' = moutputs_of e ∖ {[+ a +]}} -> a ∈ moutputs_of e.
+Proof.
+  dependent induction e; intros (e' & l & mem).
+  + cbn.
+    inversion l; subst.
+    eapply gmultiset_elem_of_disj_union. left.
+    eapply IHe1. exists p2. split.
+    eassumption. cbn in mem. multiset_solver.
+    eapply gmultiset_elem_of_disj_union. right.
+    eapply IHe2. exists q2. split.
+    eassumption. cbn in mem. multiset_solver.
+  + inversion l.
+  + inversion l.
+  + inversion l.    
+  + inversion l; subst. set_solver.
+  + destruct a. now eapply guarded_does_no_output in l.
+Qed.
+
+
+Lemma outputs_of_spec2 p a : a ∈ outputs_of p -> {q | lts p (ActExt (ActOut a)) q}.
+Proof.
+  intros mem.
+  eapply gmultiset_elem_of_dom in mem.
+  eapply mo_spec_l in mem.
+  firstorder.
+Qed.
+
+Lemma outputs_of_spec1_zero (p : proc) (a : TypeOfActions) : {q | lts p (ActExt (ActOut a)) q} 
+      -> a ∈ outputs_of p.
+Proof.    
+  intros (p' & lts__p).
+  dependent induction p.
+  + eapply gmultiset_elem_of_dom.
+    cbn. inversion lts__p; subst. apply IHp1 in H3. eapply gmultiset_elem_of_dom in H3. multiset_solver.
+     apply IHp2 in H3. eapply gmultiset_elem_of_dom in H3. multiset_solver.
+  + inversion lts__p; subst.
+  + inversion lts__p; subst.
+  + inversion lts__p; subst.
+  + inversion lts__p; subst. unfold outputs_of. multiset_solver.
+  + assert (lts g0 (ActOut a) p'). assumption. apply OutputWithValue in H.
+    decompose record H. subst. rename x into c. rename x0 into v.
+    now eapply guarded_does_no_output in lts__p.
+Qed.
+
+Lemma outputs_of_spec1 (p : proc) (a : TypeOfActions) (q : proc) : lts p (ActExt (ActOut a)) q
+      -> a ∈ outputs_of p.
+Proof.
+intros. eapply outputs_of_spec1_zero. exists q. assumption.
+Qed.
+
+Fixpoint lts_set_output (p : proc) (a : TypeOfActions) : gset proc:=
+match p with
+  | p1 ‖ p2 => 
+      let ps1 := lts_set_output p1 a in
+      let ps2 := lts_set_output p2 a in
+      (* fixme: find a way to map over sets. *)
+      list_to_set (map (fun p => p ‖ p2) (elements ps1)) ∪ list_to_set (map (fun p => p1 ‖ p) (elements ps2))
+  | pr_var _ => ∅
+  | rec _ • _ => ∅
+  | If _ Then _ Else _ => ∅
+  | c ! v • 𝟘 => if decide(a = (c ⋉ v)) then {[ (g 𝟘) ]} else ∅
+  | g _  => ∅
+end.
+
+Fixpoint lts_set_input_g (g : gproc) (a : TypeOfActions) : gset proc :=
+  match g with
+  | c ? x • p => if decide(Channel_of a = c) then {[ p^(Data_of a) ]} else ∅
+  | g1 + g2 => lts_set_input_g g1 a ∪ lts_set_input_g g2 a
+  | ① => ∅
+  | 𝟘 => ∅
+  | t • p => ∅
+  end.
+  
+Fixpoint lts_set_input (p : proc) (a : TypeOfActions) : gset proc :=
+match p with
+  | p1 ‖ p2 =>
+      let ps1 := lts_set_input p1 a in
+      let ps2 := lts_set_input p2 a in
+      list_to_set (map (fun p => p ‖ p2) (elements ps1)) ∪ list_to_set (map (fun p => p1 ‖ p) (elements ps2))
+  | pr_var _ => ∅
+  | rec _ • _ => ∅ 
+  | c ! v • 𝟘 => ∅
+  | If _ Then _ Else _ => ∅
+  | g gp => lts_set_input_g gp a  
+  end.
+  
+Fixpoint lts_set_tau_g (gp : gproc) : gset proc :=
+match gp with
+  | c ? x • p => ∅
+  | ① => ∅
+  | 𝟘 => ∅
+  | t • p => {[ p ]}
+  | gp1 + gp2 => lts_set_tau_g gp1 ∪ lts_set_tau_g gp2
+end.
+
+
+
+Fixpoint lts_set_tau (p : proc) : gset proc :=
+match p with
+  | p1 ‖ p2 =>
+      let ps1_tau : gset proc := list_to_set (map (fun p => p ‖ p2) (elements $ lts_set_tau p1)) in
+      let ps2_tau : gset proc := list_to_set (map (fun p => p1 ‖ p) (elements $ lts_set_tau p2)) in
+      let ps_tau := ps1_tau ∪ ps2_tau in
+      let acts1 := outputs_of p1 in
+      let acts2 := outputs_of p2 in
+      let ps1 :=
+        flat_map (fun a =>
+                    map
+                      (fun '(p1 , p2) => p1 ‖ p2)
+                      (list_prod (elements $ lts_set_output p1 a) (elements $ lts_set_input p2 a)))
+        (elements $ outputs_of p1) in
+      let ps2 :=
+        flat_map
+          (fun a =>
+             map
+               (fun '(p1 , p2) => p1 ‖ p2)
+               (list_prod (elements $ lts_set_input p1 a) (elements $ lts_set_output p2 a)))
+          (elements $ outputs_of p2)
+      in
+      ps_tau ∪ list_to_set ps1 ∪ list_to_set ps2
+  | c ! v • 𝟘 => ∅
+  | pr_var _ => ∅
+  | rec x • p => {[ pr_subst x p (rec x • p) ]}
+  | If C Then A Else B => match (Eval_Eq C) with 
+                          | Some true => {[ A ]}
+                          | Some false => {[ B ]}
+                          | None => ∅
+                          end
+  | g gp => lts_set_tau_g gp
+end.
+
+Lemma lts_set_output_spec0 p a q : q ∈ lts_set_output p a -> lts p (ActExt (ActOut a)) q.
+Proof.
+  intro mem.
+  dependent induction p; simpl in mem; try now inversion mem.
+  - eapply elem_of_union in mem as [mem | mem]. 
+    * eapply elem_of_list_to_set, elem_of_list_fmap in mem as (q' & eq & mem). subst.
+    apply lts_parL. apply IHp1. rewrite elem_of_elements in mem. set_solver.
+    * eapply elem_of_list_to_set, elem_of_list_fmap in mem as (q' & eq & mem). subst.
+    apply lts_parR. apply IHp2. rewrite elem_of_elements in mem. exact mem.
+  -  case (TypeOfActions_dec a (c ⋉ d)) in mem.
+    + rewrite e. rewrite e in mem.
+      destruct (decide (c ⋉ d = c ⋉ d)). subst. assert (q = (g 𝟘)). set_solver.
+      rewrite H. apply lts_output. exfalso. set_solver.
+    + destruct (decide (a = c ⋉ d)). exfalso. apply n. assumption. set_solver.
+Qed.
+
+Lemma lts_set_output_spec1 p a q : lts p (ActExt $ ActOut a) q -> q ∈ lts_set_output p a.
+Proof.
+  intro l. dependent induction l; try set_solver.
+  simpl. destruct (decide (c ⋉ v = c ⋉ v)). set_solver. exfalso. apply n. reflexivity.
+Qed.
+
+Lemma lts_set_input_spec0 p a q : q ∈ lts_set_input p a -> lts p (ActExt $ ActIn a) q.
+Proof.
+  intro mem.
+  dependent induction p; simpl in mem; try set_solver.
+  + eapply elem_of_union in mem. destruct mem.
+    ++ eapply elem_of_list_to_set in H.
+       eapply elem_of_list_fmap in H as (q' & eq & mem). subst.
+       rewrite elem_of_elements in mem. eauto with ccs.
+    ++ eapply elem_of_list_to_set in H.
+       eapply elem_of_list_fmap in H as (q' & eq & mem). subst.
+       rewrite elem_of_elements in mem. eauto with ccs.
+  + dependent induction g0; simpl in mem; try set_solver.
+      ++ destruct (decide (Channel_of a = c)).
+         +++ subst. eapply elem_of_singleton_1 in mem. subst. destruct a. simpl. apply lts_input.
+         +++ destruct a. simpl in *. inversion mem.
+      ++ eapply elem_of_union in mem. destruct mem; eauto with ccs.
+Qed.
+
+Lemma lts_set_input_spec1 p a q : lts p (ActExt $ ActIn a) q -> q ∈ lts_set_input p a.
+Proof.
+  intro l. dependent induction l; try set_solver.
+  simpl. destruct (decide (c = c)). set_solver. exfalso. apply n. reflexivity.
+Qed.
+
+
+Lemma lts_set_tau_spec0 p q : q ∈ lts_set_tau p -> lts p τ q.
+Proof.
+  - intro mem.
+    dependent induction p; simpl in mem.
+    + eapply elem_of_union in mem. destruct mem as [mem1 | mem2].
+      ++ eapply elem_of_union in mem1.
+         destruct mem1.
+         eapply elem_of_union in H as [mem1 | mem2]. 
+         eapply elem_of_list_to_set, elem_of_list_fmap in mem1 as (t' & eq & h); subst.
+         rewrite elem_of_elements in h. eauto with ccs.
+         eapply elem_of_list_to_set, elem_of_list_fmap in mem2 as (t' & eq & h); subst.
+         rewrite elem_of_elements in h. eauto with ccs.
+         eapply elem_of_list_to_set, elem_of_list_In, in_flat_map in H as (t' & eq & h); subst.
+         eapply elem_of_list_In, elem_of_list_fmap in h as ((t1 & t2) & eq' & h'). subst.
+         eapply elem_of_list_In, in_prod_iff in h' as (mem1 & mem2).
+         eapply elem_of_list_In in mem1. rewrite elem_of_elements in mem1.
+         eapply elem_of_list_In in mem2. rewrite elem_of_elements in mem2.
+         eapply lts_set_output_spec0 in mem1.
+         eapply lts_set_input_spec0 in mem2. destruct t'. eapply lts_comL. exact mem1. exact mem2.
+      ++ eapply elem_of_list_to_set, elem_of_list_In, in_flat_map in mem2 as (t' & eq & h); subst.
+         eapply elem_of_list_In, elem_of_list_fmap in h as ((t1 & t2) & eq' & h'). subst.
+         eapply elem_of_list_In, in_prod_iff in h' as (mem1 & mem2).
+         eapply elem_of_list_In in mem1. rewrite elem_of_elements in mem1.
+         eapply elem_of_list_In in mem2. rewrite elem_of_elements in mem2.
+         eapply lts_set_input_spec0 in mem1.
+         eapply lts_set_output_spec0 in mem2. destruct t'. eapply lts_comR. exact mem2. exact mem1.
+    + inversion mem.
+    + eapply elem_of_singleton_1 in mem. subst; eauto with ccs.
+    + destruct (decide (Eval_Eq e = Some true)).
+      * rewrite e0 in mem. assert (q = p1). set_solver. rewrite H. constructor. assumption.
+      * destruct (decide (Eval_Eq e = Some false)). rewrite e0 in mem. 
+        assert (q = p2). set_solver. rewrite H. constructor. assumption.
+        assert (Eval_Eq e = None). destruct (Eval_Eq e). destruct b. exfalso. apply n. reflexivity.
+        exfalso. apply n0. reflexivity. reflexivity. rewrite H in mem. set_solver.
+    + inversion mem.
+    + dependent induction g0; simpl in mem; try set_solver;
+        try eapply elem_of_singleton_1 in mem; subst; eauto with ccs.
+      eapply elem_of_union in mem as [mem1 | mem2]; eauto with ccs.
+Qed.
+
+Lemma lts_set_tau_spec1 p q : lts p τ q -> q ∈ lts_set_tau p.
+Proof. 
+  intro l. dependent induction l; simpl; try set_solver.
+  - rewrite H. set_solver. 
+  - rewrite H. set_solver. 
+  - eapply elem_of_union. left.
+    eapply elem_of_union. right.
+    eapply elem_of_list_to_set.
+    rewrite elem_of_list_In. rewrite in_flat_map.
+    exists (c ⋉ v). split.
+    + eapply elem_of_list_In, elem_of_elements.
+      eapply outputs_of_spec1_zero. eauto.
+    + eapply elem_of_list_In, elem_of_list_fmap.
+      exists (p2 , q2). split.
+      ++ reflexivity.
+      ++ eapply elem_of_list_In, in_prod_iff; split; eapply elem_of_list_In, elem_of_elements.
+         eapply lts_set_output_spec1; eauto with ccs.
+         eapply lts_set_input_spec1; eauto with ccs.
+  - eapply elem_of_union. right.
+    eapply elem_of_list_to_set.
+    rewrite elem_of_list_In. rewrite in_flat_map.
+    exists (c ⋉ v). split.
+    + eapply elem_of_list_In, elem_of_elements.
+      eapply outputs_of_spec1_zero. exists p2. exact l1.
+    + eapply elem_of_list_In, elem_of_list_fmap.
+      exists (q2 , p2). split.
+      ++ reflexivity.
+      ++ eapply elem_of_list_In, in_prod_iff; split; eapply elem_of_list_In, elem_of_elements.
+         eapply lts_set_input_spec1; eauto with ccs.
+         eapply lts_set_output_spec1; eauto with ccs.
+Qed.
+
+
+Definition lts_set (p : proc) (α : Act TypeOfActions): gset proc :=
+  match α with
+  | τ => lts_set_tau p
+  | ActExt (ActIn a) => lts_set_input p a
+  | ActExt (ActOut a) => lts_set_output p a
+  end.
+
+Lemma lts_set_spec0 p α q : q ∈ lts_set p α -> lts p α q.
+Proof.
+  destruct α as [[a|a]|].
+  - now eapply lts_set_input_spec0.
+  - now eapply lts_set_output_spec0.
+  - now eapply lts_set_tau_spec0.
+Qed.
+
+Lemma lts_set_spec1 p α q : lts p α q -> q ∈ lts_set p α.
+Proof.
+  destruct α as [[a|a]|].
+  - now eapply lts_set_input_spec1.
+  - now eapply lts_set_output_spec1.
+  - now eapply lts_set_tau_spec1.
+Qed.
+
+Definition proc_stable p α := lts_set p α = ∅.
+
+Lemma lts_dec p α q : { lts p α q } + { ~ lts p α q }.
+Proof.
+  destruct (decide (q ∈ lts_set p α)).
+  - eapply lts_set_spec0 in e. eauto.
+  - right. intro l. now eapply lts_set_spec1 in l.
+Qed.
+
+Lemma proc_stable_dec p α : Decision (proc_stable p α).
+Proof. destruct (decide (lts_set p α = ∅)); [ left | right ]; eauto. Qed.
+
+Lemma gset_nempty_ex (g : gset proc) : g ≠ ∅ -> {p | p ∈ g}.
+Proof.
+  intro n. destruct (elements g) eqn:eq.
+  + destruct n. eapply elements_empty_iff in eq. set_solver.
+  + exists p. eapply elem_of_elements. rewrite eq. set_solver.
+Qed.
 
 (* Making VACCS Instance of each class *)
 
-#[global] Program Instance VACCS_Label : Label TypeOfActions := MkLabel _ _ _.
-  Next Obligation. Admitted.
-  Next Obligation. Admitted.
+#[global] Program Instance VACCS_Label : Label TypeOfActions := 
+  {| label_eqdec := TypeOfActions_dec ;
+  label_countable := TypeOfActions_countable |}. (* useless, already said it, it is just a reminder *)
 
 #[global] Program Instance VACCS_Lts : Lts proc TypeOfActions := 
-  {| lts_step x ℓ y  := lts x ℓ y|}.
-  Next Obligation. Admitted.
-  Next Obligation. Admitted.
-  Next Obligation. Admitted.
-  Next Obligation. Admitted.
-  Next Obligation. Admitted.
-  Next Obligation. Admitted.
-  Next Obligation. Admitted.
-  Next Obligation. Admitted.
-  Next Obligation. Admitted.
+  {| lts_step x ℓ y  := lts x ℓ y ;
+     lts_state_eqdec := proc_dec ;
+     lts_step_decidable p α q := lts_dec p α q ;
+     lts_outputs := outputs_of ;
+     lts_outputs_spec1 p1 x p2 := outputs_of_spec1 p1 x p2;
+     lts_outputs_spec2 p1 x := outputs_of_spec2 p1 x;
+     lts_stable p := proc_stable p;
+     lts_stable_decidable p α := proc_stable_dec p α 
+    |}.
+    Next Obligation.
+        intros p [[a|a]|]; intro hs;eapply gset_nempty_ex in hs as (r & l); eapply lts_set_spec0 in l; 
+        exists r; assumption.
+    Qed.
+    Next Obligation.  
+        intros p [[a|a]|]; intros (q & mem); intro eq; eapply lts_set_spec1 in mem; set_solver.
+    Qed.
 
 #[global] Program Instance VACCS_LtsEq : LtsEq proc TypeOfActions := 
   {| eq_rel x y  := cgr x y;
@@ -1409,13 +2010,18 @@ Qed.
      lts_oba_output_deter p1 p2 p3 a := OBA_with_FB_Third_Axiom p1 p2 p3 a;
      lts_oba_output_tau p q1 q2 a := OBA_with_FB_Fifth_Axiom p q1 q2 a;
      lts_oba_output_deter_inv p1 p2 q1 q2 a := ExtraAxiom p1 p2 q1 q2 a;
+     lts_oba_mo p := moutputs_of p 
   |}.
-  Next Obligation. Admitted.
-  Next Obligation. Admitted.
-  Next Obligation. Admitted.
+  Next Obligation.
+    intros. simpl. unfold outputs_of.
+    now rewrite gmultiset_elem_of_dom.
+  Qed.
+  Next Obligation.
+    intros. simpl. unfold outputs_of.
+    now eapply mo_spec.
+  Qed.
+  
 
 #[global] Program Instance VACCS_LtsObaFB : LtsObaFB proc TypeOfActions :=
   {| lts_oba_fb_feedback p1 p2 p3 a := OBA_with_FB_Fourth_Axiom p1 p2 p3 a |}.
-
-
 
